First real composition running

src/tools/symbexec/examples/motor-func-test.sml
@@ -20,13 +20,43 @@ val bprog_tm = (fst o dest_eq o concl) bprog_def;
 (* motor_prep_input *)
 val birs_state_init_lbl = (snd o dest_eq o concl o EVAL) ``bir_block_pc (BL_Address (Imm32 0xb08w))``;
 val birs_stop_lbl = (snd o dest_eq o concl o EVAL) ``bir_block_pc (BL_Address (Imm32 0xb46w))``;
-val birs_stop_lbl = ``<|bpc_label := BL_Address (Imm32 0xb08w); bpc_index := 1|>``;
+val birs_stop_lbl = ``<|bpc_label := BL_Address (Imm32 0xb08w); bpc_index := 2|>``;
 
-(* TODO: *)
-val birenvtyl_def = Define `
-    birenvtyl = [("R7", BType_Imm Bit32); ("SP_process", BType_Imm Bit32); ("countw", BType_Imm Bit64)]
+(* ---------------------------------------------------------------------------------------------------------------- *)
+(* TODO: the following is copied from transfer-test script *)
+(* ---------------------------------------------------------------------------------------------------------------- *)
+val m0_mod_vars_def = Define `
+    m0_mod_vars = bmr_vars (m0_mod_bmr (T,T))
 `;
+
+val m0_mod_vars_thm = store_thm(
+   "m0_mod_vars_thm", ``
+!ef sel.
+  m0_mod_vars = bmr_vars (m0_mod_bmr (ef,sel))
+``,
+  METIS_TAC [m0_mod_vars_def, bir_lifting_machinesTheory.m0_mod_bmr_vars_EVAL]
+);
+
+val birenvtyl_def = Define `
+    birenvtyl = MAP BVarToPair m0_mod_vars
+`;
+(*    birenvtyl = [("R7", BType_Imm Bit32); ("SP_process", BType_Imm Bit32); ("countw", BType_Imm Bit64)]*)
+(*
+bir_lifting_machinesTheory.m0_mod_REGS_lifted_imms_LIST_def
+m0_mod_REGS_lifted_imms_LIST
+m0_mod_lifted_mem
+bir_lifting_machinesTheory.m0_mod_bmr_vars_EVAL
+*)
+val birenvtyl_EVAL_thm = save_thm(
+   "birenvtyl_EVAL_thm",
+  (REWRITE_CONV [birenvtyl_def, m0_mod_vars_def, bir_lifting_machinesTheory.m0_mod_bmr_vars_EVAL] THENC EVAL) ``birenvtyl``
+);
+(* ---------------------------------------------------------------------------------------------------------------- *)
+(* ---------------------------------------------------------------------------------------------------------------- *)
+
+
 (* TODO: add a sanity check here that all the variables of the program are included in birenvtyl! *)
+
 
 val birs_state_init = ``<|
   bsst_pc       := ^birs_state_init_lbl;
@@ -57,38 +87,56 @@ val tm = ``<|bsst_pc := a;
              bsst_status := BST_Running;
              bsst_pcond := c|>``;
 *)
+fun birs_get_pc tm =
+  ((snd o dest_eq o concl o EVAL) ``(^tm).bsst_pc``);
 fun birs_is_running tm =
   identical ((snd o dest_eq o concl o EVAL) ``(^tm).bsst_status``) ``BST_Running``;
 
 (*
-val symbex_A_thm = single_step_A_thm;
 val STEP_fun_spec = birs_rule_STEP_fun_spec;
+val SEQ_fun_spec = birs_rule_SEQ_fun_spec;
+
+val symbex_A_thm = single_step_A_thm;
 val stop_lbl = birs_stop_lbl;
 *)
-fun exec_until symbex_A_thm STEP_fun_spec stop_lbl =
-  (* TODO: stop condition check (create a function for this) *)
+fun exec_until (STEP_fun_spec, SEQ_fun_spec) symbex_A_thm stop_lbl =
   let
+    val _ = print ("\n");
     val (_, _, Pi_A_tm) = (symb_sound_struct_get_sysLPi_fun o concl) symbex_A_thm;
 
-    (* continue with a second step *)
+    fun is_executable st =
+      birs_is_running st andalso (not (identical (birs_get_pc st) stop_lbl));
+
     val birs_states_mid = symb_sound_struct_Pi_to_birstatelist_fun Pi_A_tm;
     val birs_states_mid_running = List.filter birs_is_running birs_states_mid;
-
-    (* TODO: *)
-    val _ = if List.length birs_states_mid_running = 1 then () else
-            raise Fail "exec_until::currently can't handle more than one running state";
-
-    (*  *)
-    val birs_state_mid = List.nth(birs_states_mid,0);
-    val single_step_B_thm = birs_rule_STEP_fun_spec birs_state_mid;
-
-    (* compose together *)
-    val bprog_composed_thm = birs_rule_SEQ_fun_spec symbex_A_thm single_step_B_thm;
+    val birs_states_mid_executable = List.filter is_executable birs_states_mid;
+    val _ = print ("- have " ^ (Int.toString (length birs_states_mid)) ^ " states\n");
+    val _ = print ("    (" ^ (Int.toString (length birs_states_mid_running)) ^ " running)\n");
+    val _ = print ("    (" ^ (Int.toString (length birs_states_mid_executable)) ^ " executable)\n");
   in
-    (* TODO: recursion *)
-    bprog_composed_thm
+    (* stop condition (no more running states, or reached the stop_lbl) *)
+    if List.length birs_states_mid_executable = 0 then
+      (print "no executable states left, terminating";
+       symbex_A_thm)
+    else
+      (* continue with a second step and then recursive call *)
+      let
+        (* select one state that did not reach the end yet *)
+        val birs_state_mid = hd birs_states_mid_executable;
+        val _ = print ("Executing one more step @(" ^ (term_to_string (birs_get_pc birs_state_mid)) ^ ")\n");
+        val single_step_B_thm = STEP_fun_spec birs_state_mid;
+
+        (* compose together *)
+        val bprog_composed_thm = SEQ_fun_spec symbex_A_thm single_step_B_thm;
+      in
+        (* recursion *)
+(*
+        exec_until (STEP_fun_spec, SEQ_fun_spec) symbex_A_thm stop_lbl (* TODO: fix *)
+*)
+        bprog_composed_thm
+      end
   end;
 (* ........................... *)
 
 
-val result = exec_until single_step_A_thm birs_rule_STEP_fun_spec birs_stop_lbl;
+val result = exec_until (birs_rule_STEP_fun_spec, birs_rule_SEQ_fun_spec) single_step_A_thm birs_stop_lbl;
